alguns updates, nada de especial

task1.dfy
@@ -12,24 +12,40 @@ class IntervalTree {
     constructor(n: int)
     requires n > 0
     ensures leaves == n
+    ensures ValidSize()
+    {
+        leaves := n;
+        tree := new int[2*(leaves-1)];
+
+    }
 
     //Updates the i-th sequence element (0-based) by v
     method update(i: int,v: int)
     requires 0 <= i < leaves
+    requires ValidSize()
+    ensures ValidSize()
+    {
+
+    }
     
     //Ranged sum over interval [a,b[
     method query(a: int,b: int) returns (r: int)
     requires 0 <= a <= b <= leaves
-    ensures r = rsum(a,b)
+    requires ValidSize()
+    ensures ValidSize()
+    ensures r == rsum(a,b)
+    {
+
+    }
 
     //Sum of elements over range [a,b[
     function rsum(a: int,b: int) : int
-    requires Valid()
+    requires ValidSize()
     decreases b-a
     requires 0 <= a <= leaves && 0 <= b <= leaves
     reads this
     {
-        if b ≤ a then 0 else get(b-1)+rsum(a,b-1)
+        if b <= a then 0 else get(b-1)+rsum(a,b-1)
     }
 
     predicate ValidSize()
@@ -43,6 +59,9 @@ class IntervalTree {
     function get(i: int) : int
     requires 0 <= i < leaves && ValidSize()
     reads this, tree
+    {
+        tree[i + leaves - 1]
+    }
 
 }
 
